Refinement/SeqDiskAPI.v
@@ -1,9 +1,20 @@
 Require Export Disk.
 Require Import Implements.
+Require Import FunctionalExtensionality.
 
 Module DSpec.
   Record State :=
     Disk { sdisk : disk }.
+
+  Lemma state_eq : forall (state state':State),
+      (forall a, sdisk state a = sdisk state' a) ->
+      state = state'.
+  Proof.
+    intros.
+    destruct state, state'; simpl in *; f_equal.
+    extensionality a.
+    eauto.
+  Qed.
 
   Definition Read a : Semantics block :=
     StepRel (fun state r state' =>
@@ -15,9 +26,8 @@ Module DSpec.
   Definition Write a b : Semantics unit :=
     StepRel (fun state r state' =>
                match sdisk state a with
-               | Some v0 => state' = Disk (upd (sdisk state) a b) /\
-                           r = tt
-               | None => True
-               end).
+               | Some v0 => state' = Disk (upd (sdisk state) a b)
+               | None => state' = state
+               end /\ r = tt).
 
 End DSpec.
